work on classify

Cedille2/Basic/Inversion.lean
@@ -5,7 +5,101 @@ import Cedille2.Basic.Weaken
 
 namespace Cedille2.Proof
 
+  inductive ConstSubExpr (sub : Const) : Term -> Prop
+  | const : sub = K -> ConstSubExpr sub (.const K)
+  | app1 : ConstSubExpr sub f -> ConstSubExpr sub (.app m f a)
+  | app2 : ConstSubExpr sub a -> ConstSubExpr sub (.app m f a)
+  | lam1 : ConstSubExpr sub A -> ConstSubExpr sub (.lam m A t)
+  | lam2 : ConstSubExpr sub t -> ConstSubExpr sub (.lam m A t)
+  | all1 : ConstSubExpr sub A -> ConstSubExpr sub (.all m A B)
+  | all2 : ConstSubExpr sub B -> ConstSubExpr sub (.all m A B)
+  | inter1 : ConstSubExpr sub T -> ConstSubExpr sub (.inter g1 g2 T t s)
+  | inter2 : ConstSubExpr sub t -> ConstSubExpr sub (.inter g1 g2 T t s)
+  | inter3 : ConstSubExpr sub s -> ConstSubExpr sub (.inter g1 g2 T t s)
+  | fst : ConstSubExpr sub t -> ConstSubExpr sub (.fst t)
+  | snd : ConstSubExpr sub t -> ConstSubExpr sub (.snd t)
+  | inter_ty1 : ConstSubExpr sub A -> ConstSubExpr sub (.inter_ty A B)
+  | inter_ty2 : ConstSubExpr sub B -> ConstSubExpr sub (.inter_ty A B)
+  | refl : ConstSubExpr sub t -> ConstSubExpr sub (.refl t)
+  | eq1 : ConstSubExpr sub a -> ConstSubExpr sub (.eq a b)
+  | eq2 : ConstSubExpr sub b -> ConstSubExpr sub (.eq a b)
+  | subst1 : ConstSubExpr sub Pr -> ConstSubExpr sub (.subst Pr e t)
+  | subst2 : ConstSubExpr sub e -> ConstSubExpr sub (.subst Pr e t)
+  | subst3 : ConstSubExpr sub t -> ConstSubExpr sub (.subst Pr e t)
+  | phi1 : ConstSubExpr sub a -> ConstSubExpr sub (.phi a b e)
+  | phi2 : ConstSubExpr sub b -> ConstSubExpr sub (.phi a b e)
+  | phi3 : ConstSubExpr sub e -> ConstSubExpr sub (.phi a b e)
+  | conv1 : ConstSubExpr sub T -> ConstSubExpr sub (.conv g1 g2 T t)
+  | conv2 : ConstSubExpr sub t -> ConstSubExpr sub (.conv g1 g2 T t)
 
+  @[simp]
+  abbrev KindNotSubExprLemma (_ : Ctx Term) : (v : JudgmentVariant) -> JudgmentIndex v -> Prop
+  | .prf => λ (t, _) => ¬ ConstSubExpr .kind t
+  | .wf => λ () => True
+
+  theorem kind_not_subexpr_lemma : Judgment v Γ ix -> KindNotSubExprLemma Γ v ix := by
+  intro j; induction j <;> simp at *
+  case _ =>
+    intro h; cases h
+    case _ h => injection h
+  case _ => intro h; cases h
+  case _ ih1 ih2 =>
+    intro h; cases h
+    case _ h => apply ih1 h
+    case _ h => apply ih2 h
+  case _ ih1 ih2 ih3 =>
+    intro h; cases h
+    case _ h => apply ih1 h
+    case _ h => apply ih3 h
+  case _ ih1 ih2 =>
+    intro h; cases h
+    case _ h => apply ih1 h
+    case _ h => apply ih2 h
+  case _ ih1 ih2 =>
+    intro h; cases h
+    case _ h => apply ih1 h
+    case _ h => apply ih2 h
+  case _ ih1 ih2 ih3 ih4 =>
+    intro h; cases h
+    case _ h => apply ih3 h
+    case _ h => apply ih1 h
+    case _ h => apply ih4 h
+  case _ ih =>
+    intro h; cases h
+    case _ h => apply ih h
+  case _ ih =>
+    intro h; cases h
+    case _ h => apply ih h
+  case _ ih1 ih2 ih3 =>
+    intro h; cases h
+    case _ h => apply ih1 h
+    case _ h => apply ih2 h
+  case _ ih1 ih2 =>
+    intro h; cases h
+    case _ h => apply ih1 h
+  case _ ih1 ih2 ih3 ih4 =>
+    intro h; cases h
+    case _ h => apply ih3 h
+    case _ h => apply ih1 h
+    case _ h => apply ih4 h
+  case _ ih1 ih2 ih3 =>
+    intro h; cases h
+    case _ h => apply ih1 h
+    case _ h => apply ih2 h
+    case _ h => apply ih3 h
+  case _ ih1 ih2 => apply ih1
+  case _ ih1 ih2 =>
+    intro h; cases h
+    case _ h => apply ih2 h
+    case _ h => apply ih1 h
+
+  theorem kind_not_subexpr : Γ ⊢ t : A -> ConstSubExpr .kind t -> False := by
+  intro h1 h2
+  have lem := kind_not_subexpr_lemma h1; simp at lem
+  apply lem h2
+
+  theorem kind_not_proof : ¬ (Γ ⊢ □ : A) := by
+  intro h; apply kind_not_subexpr h; constructor; rfl
 
   -- theorem lam_destruct_conv :
   --   Γ ⊢ .lam mf A t : T ->
