Cedille2/Basic/Classify.lean
@@ -1,0 +1,158 @@
+import Common
+import Cedille2.Proof
+import Cedille2.Basic.Weaken
+import Cedille2.Basic.Substitution
+import Cedille2.Basic.Inversion
+import Cedille2.Basic.Preservation
+
+namespace Cedille2.Proof
+
+  @[simp]
+  abbrev ClassifyKindLemmaType (_ : Ctx Term) : (v : JudgmentVariant) -> JudgmentIndex v -> Prop
+  | .prf => λ (t, A) => t.classify = .kind -> A = □
+  | .wf => λ () => True
+
+  theorem classify_kind_lemma : Judgment v Γ ix -> ClassifyKindLemmaType Γ v ix := by
+  intro j; induction j <;> simp at *
+  case var K _ _ _ _ => cases K <;> simp at *
+  case pi m K B j1 j2 ih1 ih2 =>
+    cases m <;> simp at *
+    all_goals apply ih2
+  case lam m K B t j1 j2 j3 j4 ih1 ih2 ih3 =>
+    cases m <;> simp at *
+    all_goals
+      intro h; replace ih1 := ih1 h; subst ih1
+      apply kind_not_proof j2
+  case app f m A B a B' j1 j2 j3 ih1 ih2 =>
+    cases f <;> simp at *
+    case var K _ => cases K <;> simp at *
+    case const K => cases K <;> simp at *
+    case lam m f t =>
+      split <;> simp at *
+      all_goals
+        case _ e1 e2 =>
+          split <;> try simp
+          case _ h1 =>
+            intro h2; exfalso
+            apply ih2 h2
+    case app =>
+      intro h; exfalso
+      apply ih2 h
+    case all =>
+      intro h; exfalso
+      apply ih2 h
+  case iconv t A B K j1 j2 j3 ih1 ih2 =>
+    intro h; replace ih1 := ih1 h; subst ih1
+    cases j3; case _ w r =>
+      have lem := Red.red_const_forces_const r.1; subst lem
+      replace j2 := preservation_term j2 r.2
+      exfalso; apply kind_not_proof j2
+  all_goals
+    intro h; try simp at h
+
+  theorem classify_kind : Γ ⊢ t : A -> t.classify = .kind -> A = □ := by
+  intro h1 h2; have lem := classify_kind_lemma h1; simp at lem
+  apply lem h2
+
+  @[simp]
+  abbrev ClassifyTypeLemmaType (Γ : Ctx Term) : (v : JudgmentVariant) -> JudgmentIndex v -> Prop
+  | .prf => λ (t, A) => t.classify = .type -> Γ ⊢ A : □
+  | .wf => λ () => True
+
+  theorem classify_type_lemma : Judgment v Γ ix -> ClassifyTypeLemmaType Γ v ix := by
+  intro j; induction j <;> simp at *
+  case _ K T j1 j2 ih =>
+    cases K <;> simp at *
+    subst j2; apply j1
+  case _ m K B j1 j2 ih1 ih2 =>
+    cases m <;> simp at *
+    case _ =>
+      intro h; constructor
+      apply judgment_ctx_wf j1
+    case _ =>
+      intro h; constructor
+      apply judgment_ctx_wf j1
+    case _ =>
+      intro h; replace ih2 := ih2 h
+      exfalso; apply kind_not_proof ih2
+  case _ Γ A m K B t j1 j2 j3 j4 ih1 ih2 ih3 =>
+    cases m <;> simp at *
+    case _ =>
+      intro h; replace ih3 := ih3 h
+      sorry
+    case _ =>
+      intro h; replace ih3 := ih3 h
+      sorry
+    case _ =>
+      have lem := @Judgment.pi Γ A mt K B
+      intro h; simp at lem
+      apply lem j1 j2
+  case _ Γ f m A B a B' j1 j2 j3 ih1 ih2 =>
+    intro h; cases f <;> simp at *
+    case _ => sorry
+    case _ => sorry
+    case _ => sorry
+    case _ => sorry
+    case _ => sorry
+    case _ => sorry
+    case _ => sorry
+  case _ j _ _ _ =>
+    constructor
+    apply judgment_ctx_wf j
+  case _ j _ _ _ =>
+    constructor
+    apply judgment_ctx_wf j
+  case _ j1 j2 j3 ih1 ih2 =>
+    sorry
+
+  theorem classify_type : Γ ⊢ t : A -> t.classify = .type -> Γ ⊢ A : □ := by
+  intro h1 h2; have lem := classify_type_lemma h1; simp at lem
+  apply lem h2
+
+  @[simp]
+  abbrev ClassifyTermLemmaType (Γ : Ctx Term) : (v : JudgmentVariant) -> JudgmentIndex v -> Prop
+  | .prf => λ (t, A) => t.classify = .term -> Γ ⊢ A : ★
+  | .wf => λ () => True
+
+  theorem classify_term_lemma : Judgment v Γ ix -> ClassifyTermLemmaType Γ v ix := by
+  intro j; induction j <;> simp at *
+  case _ K T j1 j2 ih =>
+    cases K <;> simp at *
+    subst j2; apply j1
+  case _ Γ A m K B j1 j2 ih1 ih2 =>
+    cases m <;> simp at *
+    case _ h =>
+      intro h; sorry
+    case _ h => sorry
+    case _ h => sorry
+  case _ Γ A m K B t j1 j2 j3 j4 ih1 ih2 ih3 =>
+    cases m <;> simp at *
+    case _ =>
+      have lem := @Judgment.pi Γ A mf K B
+      intro h; simp at lem
+      apply lem j1 j2
+    case _ =>
+      have lem := @Judgment.pi Γ A m0 K B
+      intro h; simp at lem
+      apply lem j1 j2
+    case _ => sorry
+  case _ => sorry
+  case _ j1 j2 j3 j4 j5 ih1 ih2 ih3 ih4 =>
+    apply Judgment.inter_ty j2 j3
+  case _ => sorry
+  case _ => sorry
+  case _ j1 j2 ih1 ih2 =>
+    apply Judgment.eq j1 j1 j2
+  case _ => sorry
+  case _ => sorry
+  case _ j1 j2 j3 ih1 ih2 =>
+    intro h; replace ih1 := ih1 h
+
+    sorry
+  case _ => sorry
+
+  theorem classify_term : Γ ⊢ t : A -> t.classify = .term -> Γ ⊢ A : ★ := by
+  intro h1 h2; have lem := classify_term_lemma h1; simp at lem
+  apply lem h2
+
+end Cedille2.Proof
